Had to switch bridging lemma being proved by induction from strong induction to math induction, because of interface between ambient and pRHL logics. Consequently, had to make termination metric for KEReal go down by exactly one (rather than arbitrary <). Did this by uisng KERealSimp.

smc/KeyExchange.ec
@@ -673,6 +673,130 @@ lemma ke_ideal_init :
    ={self_, adv_} ==> ={res, glob KEIdeal}].
 proof. proc; auto. qed.
 
+(* termination metric and proof for KEIdeal *)
+
+op ideal_term_metric_max : int = 4.
+
+op ideal_term_metric (st : ke_ideal_state) : int =
+     with st = KEIdealStateWaitReq1   => 4
+     with st = KEIdealStateWaitSim1 _ => 3
+     with st = KEIdealStateWaitReq2 _ => 2
+     with st = KEIdealStateWaitSim2 _ => 1
+     with st = KEIdealStateFinal    _ => 0.
+
+lemma ge0_ideal_term_metric (st : ke_ideal_state) :
+  0 <= ideal_term_metric st.
+proof. by case st. qed.
+
+lemma ideal_term_metric_is_ke_ideal_state_wait_sim1
+      (st : ke_ideal_state) :
+  is_ke_ideal_state_wait_sim1 st => ideal_term_metric st = 3.
+proof. by case st. qed.
+
+lemma ideal_term_metric_is_ke_ideal_state_wait_req2
+      (st : ke_ideal_state) :
+  is_ke_ideal_state_wait_req2 st => ideal_term_metric st = 2.
+proof. by case st. qed.
+
+lemma ideal_term_metric_is_ke_ideal_state_wait_sim2
+      (st : ke_ideal_state) :
+  is_ke_ideal_state_wait_sim2 st => ideal_term_metric st = 1.
+proof. by case st. qed.
+
+lemma ke_ideal_term_init :
+  equiv
+  [KEIdeal.init ~ KEIdeal.init :
+   ={self_, adv_} ==>
+   ={res, glob KEIdeal} /\
+   ideal_term_metric KEIdeal.st{1} = ideal_term_metric_max].
+proof. proc; auto. qed.
+
+lemma ke_ideal_term_invoke_min1 (n : int) :
+  equiv
+  [KEIdeal.invoke ~ KEIdeal.invoke :
+   ={m, glob KEIdeal} /\
+   ideal_term_metric KEIdeal.st{1} = n ==>
+   ={res, KEIdeal.st} /\
+   (res{1} = None \/ ideal_term_metric KEIdeal.st{1} = n - 1)].
+proof.
+proc; sp 3 3.
+if => //.
+inline KEIdeal.parties.
+sp 2 2.
+if => //.
+if => //.
+sp 1 1.
+if; first by move => |> &1 &2 <-.
+auto =>
+  &1 &2 [#] oget_req1_2 oget_req1_1 ->> _ ->> _ _ _ _ _ _ _
+  ->>.
+rewrite -oget_req1_2 /= in oget_req1_1.
+by elim oget_req1_1 => _ [#] -> ->.
+auto.
+auto.
+if => //.
+sp 1 1.
+if => //.
+auto.
+auto =>
+  &1 &2 [#] oget_wait_sim1_2 oget_wait_sim1_1 ->> _ ->> _ _ _ _ _ _ _
+  ->> ->>.
+rewrite -oget_wait_sim1_2 /= in oget_wait_sim1_1.
+elim oget_wait_sim1_1 => -> [#] ->.
+smt(ideal_term_metric_is_ke_ideal_state_wait_sim1).
+auto.
+if => //.
+sp 1 1.
+if => //.
+sp 1 1.
+if => //.
+auto =>
+  &1 &2 [#] oget_req2_2 oget_req2_1 oget_wait_req2_2 oget_wait_req2_1
+  ->> _ ->> _ _ _ _ _ _ _ ->> ->>.
+rewrite -oget_req2_2 /= in oget_req2_1.
+elim oget_req2_1 => _ ->.
+rewrite -oget_wait_req2_2 /= in oget_wait_req2_1.
+by elim oget_wait_req2_1 => _ [#] ->.
+auto =>
+  &1 &2 [#] oget_req2_2 oget_req2_1 oget_wait_req2_2 oget_wait_req2_1
+  ->> _ ->> _ _ _ _ _ _ _ ->> ->>.
+rewrite -oget_req2_2 /= in oget_req2_1.
+elim oget_req2_1 => _ ->.
+rewrite -oget_wait_req2_2 /= in oget_wait_req2_1.
+smt(ideal_term_metric_is_ke_ideal_state_wait_req2).
+auto.
+auto.
+if => //.
+sp 1 1.
+if => //.
+auto =>
+   &1 &2 [#] oget_wait_req2_2 oget_wait_req2_1 ->> _ ->> _ _ _ _ _ _ _
+   ->> ->>.
+rewrite -oget_wait_req2_2 in oget_wait_req2_1.
+elim oget_wait_req2_1 => -> -> ->.
+smt(ideal_term_metric_is_ke_ideal_state_wait_sim2). 
+auto.
+auto.
+qed.
+
+lemma ke_ideal_term_invoke (n : int) :
+  equiv
+  [KEIdeal.invoke ~ KEIdeal.invoke :
+   ={m, glob KEIdeal} /\
+   ideal_term_metric KEIdeal.st{1} = n ==>
+   ={res, KEIdeal.st} /\
+   (res{1} = None \/ ideal_term_metric KEIdeal.st{1} < n)].
+proof.
+conseq
+  (_ :
+   _ ==>
+   ={res, KEIdeal.st} /\
+   (res{1} = None \/ ideal_term_metric KEIdeal.st{1} = n - 1)).
+progress.
+smt(ge0_ideal_term_metric).
+apply (ke_ideal_term_invoke_min1 n).
+qed.
+
 (* Simulator *)
 
 type ke_sim_state = [
@@ -1035,6 +1159,109 @@ module KERealSimp : FUNC = {
   }
 }.
 
+lemma ke_real_simp_init :
+  equiv
+  [KERealSimp.init ~ KERealSimp.init :
+   ={self_, adv_} ==> ={glob KERealSimp}].
+proof.
+proc; auto.
+qed.
+
+(* termination metric and proof for KERealSimp *)
+
+op ke_real_simp_term_metric_max : int = 4.
+
+op ke_real_simp_term_metric (st : ke_real_simp_state) : int =
+     with st = KERealSimpStateWaitReq1   => 4
+     with st = KERealSimpStateWaitAdv1 _ => 3
+     with st = KERealSimpStateWaitReq2 _ => 2
+     with st = KERealSimpStateWaitAdv2 _ => 1
+     with st = KERealSimpStateFinal _    => 0.
+
+lemma ge0_ke_real_simp_term_metric (st : ke_real_simp_state) :
+  0 <= ke_real_simp_term_metric st.
+proof. by case st. qed.
+
+lemma ke_real_simp_term_metric_is_ke_real_simp_state_wait_adv1
+      (st : ke_real_simp_state) :
+  is_ke_real_simp_state_wait_adv1 st => ke_real_simp_term_metric st = 3.
+proof. by case st. qed.
+
+lemma ke_real_simp_term_metric_is_ke_real_simp_state_wait_req2
+      (st : ke_real_simp_state) :
+  is_ke_real_simp_state_wait_req2 st => ke_real_simp_term_metric st = 2.
+proof. by case st. qed.
+
+lemma ke_real_simp_term_metric_is_ke_real_simp_state_wait_adv2
+      (st : ke_real_simp_state) :
+  is_ke_real_simp_state_wait_adv2 st => ke_real_simp_term_metric st = 1.
+proof. by case st. qed.
+
+lemma ke_real_simp_term_init :
+  equiv
+  [KERealSimp.init ~ KERealSimp.init :
+   ={self_, adv_} ==>
+   ={res, glob KERealSimp} /\
+   ke_real_simp_term_metric KERealSimp.st{1} = ke_real_simp_term_metric_max].
+proof. proc; auto. qed.
+
+lemma ke_real_simp_term_invoke (n : int) :
+  equiv
+  [KERealSimp.invoke ~ KERealSimp.invoke :
+   ={m, glob KERealSimp} /\
+   ke_real_simp_term_metric KERealSimp.st{1} = n ==>
+   ={res, KERealSimp.st} /\
+   (res{1} = None \/ ke_real_simp_term_metric KERealSimp.st{1} = n - 1)].
+proof.
+proc; sp 3 3.
+if => //.
+inline KERealSimp.parties.
+sp 2 2.
+if => //.
+if => //.
+sp 1 1.
+if; first by move => |> &1 &2 <-.
+auto =>
+  &1 &2 [#] oget_req1_2 oget_req1_1 ->> _ ->> _ _ _ _ _ _ _
+  ->>.
+rewrite -oget_req1_2 /= in oget_req1_1.
+by elim oget_req1_1 => _ [#] -> ->.
+auto.
+auto.
+if => //.
+sp 1 1.
+if => //.
+sp 1 1.
+if; first smt().
+auto.
+auto => &1 &2 |> _ _ <- [#] -> -> ->.
+progress.
+smt(ke_real_simp_term_metric_is_ke_real_simp_state_wait_adv1).
+auto.
+auto.
+if => //.
+sp 1 1.
+if => //.
+sp 1 1.
+if; first smt().
+auto => |> &1 &2 _ _ <- [#] -> -> -> ->.
+progress.
+smt(ke_real_simp_term_metric_is_ke_real_simp_state_wait_req2).
+auto.
+auto.
+if => //.
+sp 1 1.
+if => //.
+sp 1 1.
+if; first smt().
+auto => |> &1 &2 _ _ <- [#] -> -> -> ->.
+progress.
+smt(ke_real_simp_term_metric_is_ke_real_simp_state_wait_adv2).
+auto.
+auto.
+auto.
+qed.
+
 (* relational invariant for connecting KEReal and KERealSimp *)
 
 type real_simp_rel_st = {
@@ -1121,6 +1348,26 @@ inductive real_simp_rel (st : real_simp_rel_st) =
       (real_simp_rel3 st pt1 pt2 q1 q2)
   | RealSimpRel4 (pt1 pt2 : port, q1 q2 : exp) of
       (real_simp_rel4 st pt1 pt2 q1 q2).
+
+lemma KEReal_KERealSimp_init (func adv : addr) :
+  equiv
+  [KEReal.init ~ KERealSimp.init :  
+   ={self_, adv_} /\ self_{1} = func /\ adv_{1} = adv ==>
+   KEReal.self{1} = func /\ KEReal.adv{1} = adv /\
+   Fwd1.Forw.self{1} = func ++ [1] /\ Fwd1.Forw.adv{1} = adv /\
+   Fwd2.Forw.self{1} = func ++ [2] /\ Fwd2.Forw.adv{1} = adv /\
+   KERealSimp.self{2} = func /\ KERealSimp.adv{2} = adv /\
+   real_simp_rel
+   {|real_simp_rel_st_func = func;
+     real_simp_rel_st_r1s  = KEReal.st1{1};
+     real_simp_rel_st_r2s  = KEReal.st2{1};
+     real_simp_rel_st_fws1 = Fwd1.Forw.st{1};
+     real_simp_rel_st_fws2 = Fwd2.Forw.st{1};
+     real_simp_rel_st_rss  = KERealSimp.st{2}|}].
+proof.
+proc; inline*; auto; progress.
+apply RealSimpRel0; smt().
+qed.
 
 lemma KEReal_KERealSimp_invoke (func adv : addr) :
   equiv
@@ -5749,414 +5996,4 @@ lemma ke_security
 proof.
 move => pre func_eq adv_eq.
 by apply (ke_sec Adv Env func adv &m).
-qed.
-
-(* termination metric and proof for KEReal *)
-
-type real_term_met_st = {
-  real_term_met_st_p1s  : ke_real_p1_state;
-  real_term_met_st_p2s  : ke_real_p2_state;
-  real_term_met_st_fws1 : Fwd1.fw_state;
-  real_term_met_st_fws2 : Fwd2.fw_state;
-}.
-
-op real_p1_term_metric_max : int = 2.
-
-op ke_real_p1_term_metric (st : ke_real_p1_state) : int =
-     with st = KERealP1StateWaitReq1   => 2
-     with st = KERealP1StateWaitFwd2 _ => 1
-     with st = KERealP1StateFinal _    => 0.
-
-lemma ge0_real_p1_term_metric (st : ke_real_p1_state) :
-  0 <= ke_real_p1_term_metric st.
-proof. by case st. qed.
-
-lemma real_p1_term_metric_is_ke_real_p1_state_wait_fwd2
-      (st : ke_real_p1_state) :
-  is_ke_real_p1_state_wait_fwd2 st => ke_real_p1_term_metric st = 1.
-proof. by case st. qed.
-
-op real_p2_term_metric_max : int = 2.
-
-op ke_real_p2_term_metric (st : ke_real_p2_state) : int =
-     with st = KERealP2StateWaitFwd1   => 2
-     with st = KERealP2StateWaitReq2 _ => 1
-     with st = KERealP2StateFinal _    => 0.
-
-lemma ge0_real_p2_term_metric (st : ke_real_p2_state) :
-  0 <= ke_real_p2_term_metric st.
-proof. by case st. qed.
-
-lemma real_p2_term_metric_is_ke_real_p2_state_wait_req2
-      (st : ke_real_p2_state) :
-  is_ke_real_p2_state_wait_req2 st => ke_real_p2_term_metric st = 1.
-proof. by case st. qed.
-
-op real_term_metric_max : int =
-     real_p1_term_metric_max +
-     real_p2_term_metric_max +
-     Fwd1.term_metric_max +
-     Fwd2.term_metric_max.
-
-op real_term_metric (rtms : real_term_met_st) : int =
-     ke_real_p1_term_metric rtms.`real_term_met_st_p1s +
-     ke_real_p2_term_metric rtms.`real_term_met_st_p2s +
-     Fwd1.term_metric rtms.`real_term_met_st_fws1 +
-     Fwd2.term_metric rtms.`real_term_met_st_fws2.
-
-lemma ge0_real_term_metric (rtms : real_term_met_st) :
-  0 <= real_term_metric rtms.
-proof.
-delta.
-smt(ge0_real_p1_term_metric ge0_real_p2_term_metric
-    Fwd1.ge0_term_metric Fwd2.ge0_term_metric).
-qed.
-
-lemma real_term_metric0 (rtms : real_term_met_st) :
-  real_term_metric rtms = 0 =>
-  ke_real_p1_term_metric rtms.`real_term_met_st_p1s = 0 /\
-  ke_real_p2_term_metric rtms.`real_term_met_st_p2s = 0 /\
-  Fwd1.term_metric rtms.`real_term_met_st_fws1 = 0 /\
-  Fwd2.term_metric rtms.`real_term_met_st_fws2 = 0.
-proof.
-delta.
-smt(ge0_real_p1_term_metric ge0_real_p2_term_metric
-    Fwd1.ge0_term_metric Fwd2.ge0_term_metric).
-qed.
-
-lemma ke_real_term_init :
-  equiv
-  [KEReal.init ~ KEReal.init :
-   ={self_, adv_} ==>
-   ={res, glob KEReal} /\
-   real_term_metric
-   {|real_term_met_st_p1s = KEReal.st1{1};
-     real_term_met_st_p2s = KEReal.st2{1};
-     real_term_met_st_fws1 = Fwd1.Forw.st{1};
-     real_term_met_st_fws2 = Fwd2.Forw.st{1}|} =
-   real_term_metric_max].
-proof.
-proc.
-swap [5..6] -2.
-exlim adv_{1} => adv'.
-call Fwd2.term_init.
-call Fwd1.term_init.
-auto; progress; smt().
-qed.
-
-lemma ke_real_term_invoke (n : int) :
-  equiv
-  [KEReal.invoke ~ KEReal.invoke :
-   ={m, glob KEReal} /\
-   real_term_metric
-   {|real_term_met_st_p1s = KEReal.st1{1};
-     real_term_met_st_p2s = KEReal.st2{1};
-     real_term_met_st_fws1 = Fwd1.Forw.st{1};
-     real_term_met_st_fws2 = Fwd2.Forw.st{1}|} = n ==>
-   ={res, KEReal.st1, KEReal.st2, Fwd1.Forw.st, Fwd2.Forw.st} /\
-   (res{1} = None \/
-    real_term_metric
-    {|real_term_met_st_p1s = KEReal.st1{1};
-      real_term_met_st_p2s = KEReal.st2{1};
-      real_term_met_st_fws1 = Fwd1.Forw.st{1};
-      real_term_met_st_fws2 = Fwd2.Forw.st{1}|} < n)].
-proof.
-case (n < 0).
-move => lt0_n.
-proc; exfalso; smt(ge0_real_term_metric).
-rewrite -lezNgt.
-move => ge0_n.
-proc; sp 3 3.
-if => //.
-inline KEReal.loop.
-sp 3 3; wp.
-conseq
-  (_ :
-   ={not_done, m0, glob KEReal, glob Fwd1.Forw, glob Fwd2.Forw} /\
-   not_done{1} /\
-   real_term_metric
-   {|real_term_met_st_p1s = KEReal.st1{1};
-     real_term_met_st_p2s = KEReal.st2{1};
-     real_term_met_st_fws1 = Fwd1.Forw.st{1};
-     real_term_met_st_fws2 = Fwd2.Forw.st{1};|} = n ==>
-   _) => //.
-move : ge0_n.
-elim n.
-rcondt{1} 1; first auto.
-rcondt{2} 1; first auto.
-if => //.
-inline{1} (1) KEReal.party1.
-inline{2} (1) KEReal.party1.
-rcondf{1} 3; first auto; smt(real_term_metric0).
-rcondf{2} 3; first auto; smt(real_term_metric0).
-rcondf{1} 3; first auto;
-  smt(real_term_metric0 real_p1_term_metric_is_ke_real_p1_state_wait_fwd2).
-rcondf{2} 3; first auto;
-  smt(real_term_metric0 real_p1_term_metric_is_ke_real_p1_state_wait_fwd2).
-rcondt{1} 4; first auto.
-rcondt{2} 4; first auto.
-rcondf{1} 5; first auto.
-rcondf{2} 5; first auto.
-auto.
-if => //.
-inline{1} (1) KEReal.party2.
-inline{2} (1) KEReal.party2.
-rcondf{1} 3; first auto; smt(real_term_metric0).
-rcondf{2} 3; first auto; smt(real_term_metric0).
-rcondf{1} 3; first auto;
-  smt(real_term_metric0 real_p2_term_metric_is_ke_real_p2_state_wait_req2).
-rcondf{2} 3; first auto;
-  smt(real_term_metric0 real_p2_term_metric_is_ke_real_p2_state_wait_req2).
-rcondt{1} 4; first auto.
-rcondt{2} 4; first auto.
-rcondf{1} 5; first auto.
-rcondf{2} 5; first auto.
-auto.
-if => //.
-seq 1 1 :
-  (={not_done, r0, glob KEReal, glob Fwd1.Forw, glob Fwd2.Forw} /\
-   r0{1} = None).
-call (Fwd1.term_invoke 0).
-auto; progress; smt(real_term_metric0 Fwd1.ge0_term_metric).
-rcondt{1} 1; first auto.
-rcondt{2} 1; first auto.
-rcondf{1} 2; first auto.
-rcondf{2} 2; first auto.
-auto.
-seq 1 1 :
-  (={not_done, r0, glob KEReal, glob Fwd1.Forw, glob Fwd2.Forw} /\
-   r0{1} = None).
-call (Fwd2.term_invoke 0).
-auto; progress; smt(real_term_metric0 Fwd2.ge0_term_metric).
-rcondt{1} 1; first auto.
-rcondt{2} 1; first auto.
-rcondf{1} 2; first auto.
-rcondf{2} 2; first auto.
-auto.
-move => n ge0_n IH.
-rcondt{1} 1; first auto.
-rcondt{2} 1; first auto.
-seq 1 1 :
-   (={not_done, m0, r0, glob KEReal, glob Fwd1.Forw, glob Fwd2.Forw} /\
-    not_done{1} /\
-    (r0{1} = None \/
-     real_term_metric
-     {|real_term_met_st_p1s = KEReal.st1{1};
-       real_term_met_st_p2s = KEReal.st2{1};
-       real_term_met_st_fws1 = Fwd1.Forw.st{1};
-       real_term_met_st_fws2 = Fwd2.Forw.st{1};|} = n)).
-if => //.
-inline KEReal.party1.
-sp 2 2.
-if => //.
-if => //.
-sp 1 1.
-if; first by move => &1 &2 |> <-.
-auto => &1 &2 |> <-; smt().
-auto.
-auto.
-if => //.
-sp 1 1.
-if => //.
-sp 1 1.
-if.
-move => &1 &2 [#] oget_dec_fw_rsp2 oget_dec_fw_rsp1 _ _ ->> _
-        ->> _ _ ->>.
-rewrite -oget_dec_fw_rsp2 /= in oget_dec_fw_rsp1.
-by elim oget_dec_fw_rsp1.
-auto => |> &1 &2 <- [#] _ _ _ -> <- [#] -> -> -> _ /=.
-rewrite /real_term_metric /=.
-smt(real_p1_term_metric_is_ke_real_p1_state_wait_fwd2).
-auto.
-auto.
-auto.
-inline KEReal.party2.
-if => //.
-sp 2 2.
-if => //.
-if => //.
-sp 1 1.
-if.
-move =>
-  &1 &2 [#] oget_dec_fw_rsp2 oget_dec_fw_rsp1 ->> _ ->> _ _ ->>.
-rewrite -oget_dec_fw_rsp2 /= in oget_dec_fw_rsp1.
-by elim oget_dec_fw_rsp1.
-auto => &1 &2 |> <-; smt().
-auto.
-auto.
-if => //.
-sp 1 1.
-if => //.
-sp 1 1.
-if => //.
-move =>
-  &1 &2 [#] oget_dec_fw_rsp2 oget_dec_fw_rsp1
-  oget_dec_wait_req2_2 oget_dec_wait_req2_1
-  ->> _ ->> _ _ ->> ->>.
-rewrite -oget_dec_fw_rsp2 /= in oget_dec_fw_rsp1.
-elim oget_dec_fw_rsp1.
-rewrite -oget_dec_wait_req2_2 /= in oget_dec_wait_req2_1.
-by elim oget_dec_wait_req2_1.
-auto => &1 &2 |> <- [#] _ -> <-.
-progress.
-smt(real_p2_term_metric_is_ke_real_p2_state_wait_req2).
-auto.
-auto.
-auto.
-if => //.
-exlim (Fwd1.term_metric Fwd1.Forw.st{1}) => m.
-call (Fwd1.term_invoke m).
-auto.
-auto; progress; smt().
-exlim (Fwd2.term_metric Fwd2.Forw.st{1}) => m.
-call (Fwd2.term_invoke m).
-auto.
-auto; progress; smt().
-if => //.
-rcondf{1} 2; first auto.
-rcondf{2} 2; first auto.
-auto; progress; smt().
-sp 1 1.
-conseq
-  (_ :
-    ={not_done, m0, glob KEReal, glob Fwd1.Forw, glob Fwd2.Forw} /\
-    not_done{1} /\
-    real_term_metric
-    {|real_term_met_st_p1s = KEReal.st1{1};
-      real_term_met_st_p2s = KEReal.st2{1};
-      real_term_met_st_fws1 = Fwd1.Forw.st{1};
-      real_term_met_st_fws2 = Fwd2.Forw.st{1};|} = n ==>
-    ={r0, KEReal.st1, KEReal.st2, Fwd1.Forw.st, Fwd2.Forw.st} /\
-    (r0{1} = None \/
-     real_term_metric
-     {|real_term_met_st_p1s = KEReal.st1{1};
-       real_term_met_st_p2s = KEReal.st2{1};
-       real_term_met_st_fws1 = Fwd1.Forw.st{1};
-       real_term_met_st_fws2 = Fwd2.Forw.st{1};|} < n)) => //.
-progress; smt().
-progress; smt().
-qed.
-
-(* termination metric and proof for KEIdeal *)
-
-op ideal_term_metric_max : int = 4.
-
-op ideal_term_metric (st : ke_ideal_state) : int =
-     with st = KEIdealStateWaitReq1   => 4
-     with st = KEIdealStateWaitSim1 _ => 3
-     with st = KEIdealStateWaitReq2 _ => 2
-     with st = KEIdealStateWaitSim2 _ => 1
-     with st = KEIdealStateFinal    _ => 0.
-
-lemma ge0_ideal_term_metric (st : ke_ideal_state) :
-  0 <= ideal_term_metric st.
-proof. by case st. qed.
-
-lemma ideal_term_metric_is_ke_ideal_state_wait_sim1
-      (st : ke_ideal_state) :
-  is_ke_ideal_state_wait_sim1 st => ideal_term_metric st = 3.
-proof. by case st. qed.
-
-lemma ideal_term_metric_is_ke_ideal_state_wait_req2
-      (st : ke_ideal_state) :
-  is_ke_ideal_state_wait_req2 st => ideal_term_metric st = 2.
-proof. by case st. qed.
-
-lemma ideal_term_metric_is_ke_ideal_state_wait_sim2
-      (st : ke_ideal_state) :
-  is_ke_ideal_state_wait_sim2 st => ideal_term_metric st = 1.
-proof. by case st. qed.
-
-lemma ke_ideal_term_init :
-  equiv
-  [KEIdeal.init ~ KEIdeal.init :
-   ={self_, adv_} ==>
-   ={res, glob KEIdeal} /\
-   ideal_term_metric KEIdeal.st{1} = ideal_term_metric_max].
-proof. proc; auto. qed.
-
-lemma ke_ideal_term_invoke_min1 (n : int) :
-  equiv
-  [KEIdeal.invoke ~ KEIdeal.invoke :
-   ={m, glob KEIdeal} /\
-   ideal_term_metric KEIdeal.st{1} = n ==>
-   ={res, KEIdeal.st} /\
-   (res{1} = None \/ ideal_term_metric KEIdeal.st{1} = n - 1)].
-proof.
-proc; sp 3 3.
-if => //.
-inline KEIdeal.parties.
-sp 2 2.
-if => //.
-if => //.
-sp 1 1.
-if; first by move => |> &1 &2 <-.
-auto =>
-  &1 &2 [#] oget_req1_2 oget_req1_1 ->> _ ->> _ _ _ _ _ _ _
-  ->>.
-rewrite -oget_req1_2 /= in oget_req1_1.
-by elim oget_req1_1 => _ [#] -> ->.
-auto.
-auto.
-if => //.
-sp 1 1.
-if => //.
-auto.
-auto =>
-  &1 &2 [#] oget_wait_sim1_2 oget_wait_sim1_1 ->> _ ->> _ _ _ _ _ _ _
-  ->> ->>.
-rewrite -oget_wait_sim1_2 /= in oget_wait_sim1_1.
-elim oget_wait_sim1_1 => -> [#] ->.
-smt(ideal_term_metric_is_ke_ideal_state_wait_sim1).
-auto.
-if => //.
-sp 1 1.
-if => //.
-sp 1 1.
-if => //.
-auto =>
-  &1 &2 [#] oget_req2_2 oget_req2_1 oget_wait_req2_2 oget_wait_req2_1
-  ->> _ ->> _ _ _ _ _ _ _ ->> ->>.
-rewrite -oget_req2_2 /= in oget_req2_1.
-elim oget_req2_1 => _ ->.
-rewrite -oget_wait_req2_2 /= in oget_wait_req2_1.
-by elim oget_wait_req2_1 => _ [#] ->.
-auto =>
-  &1 &2 [#] oget_req2_2 oget_req2_1 oget_wait_req2_2 oget_wait_req2_1
-  ->> _ ->> _ _ _ _ _ _ _ ->> ->>.
-rewrite -oget_req2_2 /= in oget_req2_1.
-elim oget_req2_1 => _ ->.
-rewrite -oget_wait_req2_2 /= in oget_wait_req2_1.
-smt(ideal_term_metric_is_ke_ideal_state_wait_req2).
-auto.
-auto.
-if => //.
-sp 1 1.
-if => //.
-auto =>
-   &1 &2 [#] oget_wait_req2_2 oget_wait_req2_1 ->> _ ->> _ _ _ _ _ _ _
-   ->> ->>.
-rewrite -oget_wait_req2_2 in oget_wait_req2_1.
-elim oget_wait_req2_1 => -> -> ->.
-smt(ideal_term_metric_is_ke_ideal_state_wait_sim2). 
-auto.
-auto.
-qed.
-
-lemma ke_ideal_term_invoke (n : int) :
-  equiv
-  [KEIdeal.invoke ~ KEIdeal.invoke :
-   ={m, glob KEIdeal} /\
-   ideal_term_metric KEIdeal.st{1} = n ==>
-   ={res, KEIdeal.st} /\
-   (res{1} = None \/ ideal_term_metric KEIdeal.st{1} < n)].
-proof.
-conseq
-  (_ :
-   _ ==>
-   ={res, KEIdeal.st} /\
-   (res{1} = None \/ ideal_term_metric KEIdeal.st{1} = n - 1)).
-progress.
-smt(ge0_ideal_term_metric).
-apply (ke_ideal_term_invoke_min1 n).
 qed.
